more symbols;

thys/MiniML/Instance.thy
@@ -20,13 +20,13 @@ primrec bound_scheme_inst :: "[nat => type_scheme, type_scheme] => type_scheme" 
 | "bound_scheme_inst S (sch1 =-> sch2) = ((bound_scheme_inst S sch1) =-> (bound_scheme_inst S sch2))"
   
 definition is_bound_typ_instance :: "[typ, type_scheme] => bool"  (infixr "<|" 70) where
-  is_bound_typ_instance: "t <| sch = (? S. t = (bound_typ_inst S sch))"
+  is_bound_typ_instance: "t <| sch = (\<exists>S. t = (bound_typ_inst S sch))"
 
 instantiation type_scheme :: ord
 begin
 
 definition
-  le_type_scheme_def: "sch' <= (sch::type_scheme) \<longleftrightarrow> (!t. t <| sch' --> t <| sch)"
+  le_type_scheme_def: "sch' \<le> (sch::type_scheme) \<longleftrightarrow> (\<forall>t. t <| sch' \<longrightarrow> t <| sch)"
 
 definition
   "(sch' < (sch :: type_scheme)) \<longleftrightarrow> sch' \<le> sch \<and> sch' \<noteq> sch"
@@ -43,7 +43,7 @@ instantiation list :: (ord) ord
 begin
 
 definition
-  le_env_def: "A \<le> B \<longleftrightarrow> length B = length A \<and> (!i. i < length A --> A!i <= B!i)"
+  le_env_def: "A \<le> B \<longleftrightarrow> length B = length A \<and> (\<forall>i. i < length A \<longrightarrow> A!i \<le> B!i)"
 
 definition
   "(A < (B :: 'a list)) \<longleftrightarrow> A \<le> B \<and> A \<noteq> B"
@@ -58,22 +58,22 @@ lemma bound_typ_inst_mk_scheme [simp]: "bound_typ_inst S (mk_scheme t) = t"
   by (induct t) simp_all
 
 lemma bound_typ_inst_composed_subst [simp]:
-    "bound_typ_inst ($S o R) ($S sch) = $S (bound_typ_inst R sch)"
+    "bound_typ_inst ($S \<circ> R) ($S sch) = $S (bound_typ_inst R sch)"
   by (induct sch) simp_all
 
 lemma bound_typ_inst_eq:
-    "S = S' ==> sch = sch' ==> bound_typ_inst S sch = bound_typ_inst S' sch'"
+    "S = S' \<Longrightarrow> sch = sch' \<Longrightarrow> bound_typ_inst S sch = bound_typ_inst S' sch'"
   by simp
 
 lemma bound_scheme_inst_mk_scheme [simp]:
     "bound_scheme_inst B (mk_scheme t) = mk_scheme t"
   by (induct t) simp_all
 
-lemma substitution_lemma: "$S (bound_scheme_inst B sch) = (bound_scheme_inst ($S o B) ($ S sch))"
+lemma substitution_lemma: "$S (bound_scheme_inst B sch) = (bound_scheme_inst ($S \<circ> B) ($ S sch))"
   by (induct sch) simp_all
 
-lemma bound_scheme_inst_type [rule_format]: "!t. mk_scheme t = bound_scheme_inst B sch -->  
-          (? S. !x:bound_tv sch. B x = mk_scheme (S x))"
+lemma bound_scheme_inst_type [rule_format]: "\<forall>t. mk_scheme t = bound_scheme_inst B sch \<longrightarrow>  
+          (\<exists>S. \<forall>x\<in>bound_tv sch. B x = mk_scheme (S x))"
 apply (induct_tac "sch")
 apply (simp (no_asm))
 apply safe
@@ -91,60 +91,60 @@ apply (drule sym)
 apply (drule mp, fast)+
 apply safe
 apply (rename_tac S1 S2)
-apply (rule_tac x = "%x. if x:bound_tv type_scheme1 then (S1 x) else (S2 x) " in exI)
+apply (rule_tac x = "\<lambda>x. if x:bound_tv type_scheme1 then (S1 x) else (S2 x) " in exI)
 apply auto
 done
 
 lemma subst_to_scheme_inverse: 
   "new_tv n sch \<Longrightarrow>
-    subst_to_scheme (%k. if n <= k then BVar (k - n) else FVar k)  
-      (bound_typ_inst (%k. TVar (k + n)) sch) = sch"
+    subst_to_scheme (\<lambda>k. if n \<le> k then BVar (k - n) else FVar k)  
+      (bound_typ_inst (\<lambda>k. TVar (k + n)) sch) = sch"
   apply (induct sch)
     apply (simp add: not_le)
    apply (simp add: le_add2 diff_add_inverse2)
   apply simp
   done
 
-lemma aux: "t = t' ==>  
-      subst_to_scheme (%k. if n <= k then BVar (k - n) else FVar k) t =  
-      subst_to_scheme (%k. if n <= k then BVar (k - n) else FVar k) t'"
+lemma aux: "t = t' \<Longrightarrow>  
+      subst_to_scheme (\<lambda>k. if n \<le> k then BVar (k - n) else FVar k) t =  
+      subst_to_scheme (\<lambda>k. if n \<le> k then BVar (k - n) else FVar k) t'"
   by blast
 
 lemma aux2: "new_tv n sch \<Longrightarrow>
-  subst_to_scheme (%k. if n <= k then BVar (k - n) else FVar k) (bound_typ_inst S sch) =  
-    bound_scheme_inst ((subst_to_scheme (%k. if n <= k then BVar (k - n) else FVar k)) o S) sch"
+  subst_to_scheme (\<lambda>k. if n \<le> k then BVar (k - n) else FVar k) (bound_typ_inst S sch) =  
+    bound_scheme_inst ((subst_to_scheme (\<lambda>k. if n \<le> k then BVar (k - n) else FVar k)) \<circ> S) sch"
     by (induct sch) auto
 
 lemma le_type_scheme_def2:
   fixes sch sch' :: type_scheme
-  shows "(sch' <= sch) = (? B. sch' = bound_scheme_inst B sch)"
+  shows "(sch' \<le> sch) = (\<exists>B. sch' = bound_scheme_inst B sch)"
 apply (unfold le_type_scheme_def is_bound_typ_instance)
 apply (rule iffI)
 apply (cut_tac sch = "sch" in fresh_variable_type_schemes)
 apply (cut_tac sch = "sch'" in fresh_variable_type_schemes)
 apply (drule make_one_new_out_of_two)
 apply assumption
-apply (erule_tac V = "? n. new_tv n sch'" in thin_rl)
+apply (erule_tac V = "\<exists>n. new_tv n sch'" in thin_rl)
 apply (erule exE)
 apply (erule allE)
 apply (drule mp)
-apply (rule_tac x = " (%k. TVar (k + n))" in exI)
+apply (rule_tac x = " (\<lambda>k. TVar (k + n))" in exI)
 apply (rule refl)
 apply (erule exE)
 apply (erule conjE)+
 apply (drule_tac n = "n" in aux)
 apply (simp add: subst_to_scheme_inverse)
-apply (rule_tac x = " (subst_to_scheme (%k. if n <= k then BVar (k - n) else FVar k)) o S" in exI)
+apply (rule_tac x = " (subst_to_scheme (\<lambda>k. if n \<le> k then BVar (k - n) else FVar k)) \<circ> S" in exI)
 apply (simp (no_asm_simp) add: aux2)
 apply safe
-apply (rule_tac x = "%n. bound_typ_inst S (B n) " in exI)
+apply (rule_tac x = "\<lambda>n. bound_typ_inst S (B n) " in exI)
 apply (induct_tac "sch")
 apply (simp (no_asm))
 apply (simp (no_asm))
 apply (simp (no_asm_simp))
 done
 
-lemma le_type_eq_is_bound_typ_instance [rule_format]: "(mk_scheme t) <= sch = t <| sch"
+lemma le_type_eq_is_bound_typ_instance [rule_format]: "(mk_scheme t) \<le> sch = t <| sch"
 apply (unfold is_bound_typ_instance)
 apply (simp (no_asm) add: le_type_scheme_def2)
 apply (rule iffI)
@@ -173,7 +173,7 @@ apply simp
 done
 
 lemma le_env_Cons [iff]: 
-  "(sch # A <= sch' # B) = (sch <= (sch'::type_scheme) & A <= B)"
+  "(sch # A \<le> sch' # B) = (sch \<le> (sch'::type_scheme) \<and> A \<le> B)"
 apply (unfold le_env_def)
 apply (simp (no_asm))
 apply (rule iffI)
@@ -192,18 +192,18 @@ apply (induct_tac "i")
 apply simp_all
 done
 
-lemma is_bound_typ_instance_closed_subst: "t <| sch ==> $S t <| $S sch"
+lemma is_bound_typ_instance_closed_subst: "t <| sch \<Longrightarrow> $S t <| $S sch"
 apply (unfold is_bound_typ_instance)
 apply (erule exE)
 apply (rename_tac "SA") 
 apply simp
-apply (rule_tac x = "$S o SA" in exI)
+apply (rule_tac x = "$S \<circ> SA" in exI)
 apply simp
 done
 
 lemma S_compatible_le_scheme:
   fixes sch sch' :: type_scheme
-  shows "sch' <= sch ==> $S sch' <= $ S sch"
+  shows "sch' \<le> sch \<Longrightarrow> $S sch' \<le> $ S sch"
 apply (simp add: le_type_scheme_def2)
 apply (erule exE)
 apply (simp add: substitution_lemma)
@@ -212,38 +212,38 @@ done
 
 lemma S_compatible_le_scheme_lists: 
   fixes A A' :: "type_scheme list"
-  shows "A' <= A ==> $S A' <= $ S A"
+  shows "A' \<le> A \<Longrightarrow> $S A' \<le> $ S A"
 apply (unfold le_env_def app_subst_list)
 apply (simp cong add: conj_cong)
 apply (fast intro!: S_compatible_le_scheme)
 done
 
-lemma bound_typ_instance_trans: "[| t <| sch; sch <= sch' |] ==> t <| sch'"
+lemma bound_typ_instance_trans: "[| t <| sch; sch \<le> sch' |] ==> t <| sch'"
   unfolding le_type_scheme_def by blast
 
-lemma le_type_scheme_refl [iff]: "sch <= (sch::type_scheme)"
+lemma le_type_scheme_refl [iff]: "sch \<le> (sch::type_scheme)"
   unfolding le_type_scheme_def by blast
 
-lemma le_env_refl [iff]: "A <= (A::type_scheme list)"
+lemma le_env_refl [iff]: "A \<le> (A::type_scheme list)"
   unfolding le_env_def by blast
 
-lemma bound_typ_instance_BVar [iff]: "sch <= BVar n"
+lemma bound_typ_instance_BVar [iff]: "sch \<le> BVar n"
 apply (unfold le_type_scheme_def is_bound_typ_instance)
 apply (intro strip)
-apply (rule_tac x = "%a. t" in exI)
+apply (rule_tac x = "\<lambda>a. t" in exI)
 apply simp
 done
 
-lemma le_FVar [simp]: "(sch <= FVar n) = (sch = FVar n)"
+lemma le_FVar [simp]: "(sch \<le> FVar n) = (sch = FVar n)"
 apply (unfold le_type_scheme_def is_bound_typ_instance)
 apply (induct_tac "sch")
 apply auto
 done
 
-lemma not_FVar_le_Fun [iff]: "~(FVar n <= sch1 =-> sch2)"
+lemma not_FVar_le_Fun [iff]: "~(FVar n \<le> sch1 =-> sch2)"
   unfolding le_type_scheme_def is_bound_typ_instance by simp
 
-lemma not_BVar_le_Fun [iff]: "~(BVar n <= sch1 =-> sch2)"
+lemma not_BVar_le_Fun [iff]: "~(BVar n \<le> sch1 =-> sch2)"
 apply (unfold le_type_scheme_def is_bound_typ_instance)
 apply simp
 apply (rule_tac x = "TVar n" in exI)
@@ -251,14 +251,14 @@ apply fastforce
 done
 
 lemma Fun_le_FunD: 
-  "(sch1 =-> sch2 <= sch1' =-> sch2') ==> sch1 <= sch1' & sch2 <= sch2'"
+  "(sch1 =-> sch2 \<le> sch1' =-> sch2') \<Longrightarrow> sch1 \<le> sch1' \<and> sch2 \<le> sch2'"
   unfolding le_type_scheme_def is_bound_typ_instance by fastforce
 
-lemma scheme_le_Fun: "(sch' <= sch1 =-> sch2) \<Longrightarrow> ? sch'1 sch'2. sch' = sch'1 =-> sch'2"
+lemma scheme_le_Fun: "(sch' \<le> sch1 =-> sch2) \<Longrightarrow> \<exists>sch'1 sch'2. sch' = sch'1 =-> sch'2"
   by (induct sch') auto
 
 lemma le_type_scheme_free_tv [rule_format]:
-  "!sch'::type_scheme. sch <= sch' --> free_tv sch' <= free_tv sch"
+  "\<forall>sch'::type_scheme. sch \<le> sch' \<longrightarrow> free_tv sch' \<le> free_tv sch"
 apply (induct_tac "sch")
   apply (rule allI)
   apply (induct_tac "sch'")
@@ -281,7 +281,7 @@ apply fast
 done
 
 lemma le_env_free_tv [rule_format]:
-  "!A::type_scheme list. A <= B --> free_tv B <= free_tv A"
+  "\<forall>A::type_scheme list. A \<le> B \<longrightarrow> free_tv B \<le> free_tv A"
 apply (induct_tac "B")
  apply (simp (no_asm))
 apply (rule allI)
