thys/MiniML/Maybe.thy
@@ -15,7 +15,7 @@ definition
   "option_bind m f = (case m of None => None | Some r => f r)"
 
 syntax "_option_bind" :: "[pttrns,'a option,'b] => 'c" ("(_ := _;//_)" 0)
-translations "P := E; F" == "CONST option_bind E (%P. F)"
+translations "P := E; F" == "CONST option_bind E (\<lambda>P. F)"
 
 
 \<comment> \<open>constructor laws for @{text option_bind}\<close>
@@ -29,12 +29,12 @@ declare option_bind_Some [simp] option_bind_None [simp]
 
 \<comment> \<open>expansion of @{text option_bind}\<close>
 lemma split_option_bind: "P(option_bind res f) =  
-          ((res = None --> P None) & (!s. res = Some s --> P(f s)))"
+          ((res = None \<longrightarrow> P None) \<and> (\<forall>s. res = Some s \<longrightarrow> P(f s)))"
   unfolding option_bind_def
   by (rule option.split)
 
 lemma option_bind_eq_None [simp]:
-    "((option_bind m f) = None) = ((m=None) | (? p. m = Some p & f p = None))"
+    "((option_bind m f) = None) = ((m=None) | (\<exists>p. m = Some p \<and> f p = None))"
   by (simp split: split_option_bind)
 
 lemma rotate_Some: "(y = Some x) = (Some x = y)"
