thys/MiniML/Type.thy
@@ -111,17 +111,17 @@ text
    occurring in the type structure *}
 definition
   new_tv :: "[nat,'a::type_struct] => bool" where
-  "new_tv n ts = (! m. m:(free_tv ts) --> m<n)"
+  "new_tv n ts = (\<forall>m. m:(free_tv ts) \<longrightarrow> m<n)"
 
 \<comment> \<open>identity\<close>
 definition
   id_subst :: subst where
-  "id_subst = (%n. TVar n)"
+  "id_subst = (\<lambda>n. TVar n)"
 
 \<comment> \<open>domain of a substitution\<close>
 definition
   dom :: "subst => nat set" where
-  "dom S = {n. S n ~= TVar n}" 
+  "dom S = {n. S n \<noteq> TVar n}" 
 
 \<comment> \<open>codomain of a substitution: the introduced variables\<close>
 definition
@@ -170,21 +170,21 @@ lemma free_tv_subst:
 
 \<comment> \<open>unification algorithm mgu\<close>
 axiomatization mgu :: "typ \<Rightarrow> typ \<Rightarrow> subst option" where
-  mgu_eq:   "mgu t1 t2 = Some U ==> $U t1 = $U t2"
-  and mgu_mg:   "[| (mgu t1 t2) = Some U; $S t1 = $S t2 |] ==> ? R. S = $R o U"
-  and mgu_Some: "$S t1 = $S t2 ==> ? U. mgu t1 t2 = Some U"
-  and mgu_free: "mgu t1 t2 = Some U ==> (free_tv U) <= (free_tv t1) Un (free_tv t2)"
+  mgu_eq:   "mgu t1 t2 = Some U \<Longrightarrow> $U t1 = $U t2"
+  and mgu_mg:   "[| (mgu t1 t2) = Some U; $S t1 = $S t2 |] ==> \<exists>R. S = $R \<circ> U"
+  and mgu_Some: "$S t1 = $S t2 \<Longrightarrow> \<exists>U. mgu t1 t2 = Some U"
+  and mgu_free: "mgu t1 t2 = Some U \<Longrightarrow> (free_tv U) \<subseteq> (free_tv t1) Un (free_tv t2)"
 
 
 declare mgu_eq [simp] mgu_mg [simp] mgu_free [simp]
-lemma mk_scheme_Fun [rule_format]: "mk_scheme t = sch1 =-> sch2 --> (? t1 t2. sch1 = mk_scheme t1 & sch2 = mk_scheme t2)"
+lemma mk_scheme_Fun [rule_format]: "mk_scheme t = sch1 =-> sch2 \<longrightarrow> (\<exists>t1 t2. sch1 = mk_scheme t1 \<and> sch2 = mk_scheme t2)"
 apply (induct_tac "t")
 apply (simp (no_asm))
 apply simp
 apply fast
 done
 
-lemma mk_scheme_injective [rule_format]: "!t'. mk_scheme t = mk_scheme t' --> t=t'"
+lemma mk_scheme_injective [rule_format]: "\<forall>t'. mk_scheme t = mk_scheme t' \<longrightarrow> t=t'"
 apply (induct_tac "t")
  apply (rule allI)
  apply (induct_tac "t'")
@@ -251,13 +251,13 @@ apply (simp (no_asm))
 done
 
 lemma new_tv_Fun: 
-  "new_tv n (t1 -> t2) = (new_tv n t1 & new_tv n t2)"
+  "new_tv n (t1 -> t2) = (new_tv n t1 \<and> new_tv n t2)"
 apply (unfold new_tv_def)
 apply (fastforce)
 done
 
 lemma new_tv_Fun2: 
-  "new_tv n (t1 =-> t2) = (new_tv n t1 & new_tv n t2)"
+  "new_tv n (t1 =-> t2) = (new_tv n t1 \<and> new_tv n t2)"
 apply (unfold new_tv_def)
 apply (fastforce)
 done
@@ -269,7 +269,7 @@ apply (simp (no_asm))
 done
 
 lemma new_tv_Cons: 
-  "new_tv n (x#l) = (new_tv n x & new_tv n l)"
+  "new_tv n (x#l) = (new_tv n x \<and> new_tv n l)"
 apply (unfold new_tv_def)
 apply (fastforce)
 done
@@ -289,11 +289,11 @@ lemma new_tv_id_subst [simp]: "new_tv n id_subst"
   by (simp add: id_subst_def new_tv_def free_tv_subst dom_def cod_def)
 
 lemma new_if_subst_type_scheme [simp]: "new_tv n (sch::type_scheme) \<Longrightarrow>
-    $(%k. if k<n then S k else S' k) sch = $S sch"
+    $(\<lambda>k. if k<n then S k else S' k) sch = $S sch"
   by (induct sch) simp_all
 
 lemma new_if_subst_type_scheme_list [simp]: "new_tv n (A::type_scheme list) \<Longrightarrow>
-    $(%k. if k<n then S k else S' k) A = $S A"
+    $(\<lambda>k. if k<n then S k else S' k) A = $S A"
   by (induct A) simp_all
 
 
@@ -310,7 +310,7 @@ lemma free_tv_id_subst [simp]: "free_tv id_subst = {}"
   unfolding free_tv_subst by simp
 
 lemma free_tv_nth_A_impl_free_tv_A [rule_format, simp]:
-  "!n. n < length A --> x : free_tv (A!n) --> x : free_tv A"
+  "\<forall>n. n < length A \<longrightarrow> x : free_tv (A!n) \<longrightarrow> x : free_tv A"
 apply (induct A)
 apply simp
 apply (rule allI)
@@ -320,7 +320,7 @@ apply simp
 done
 
 lemma free_tv_nth_nat_A [rule_format]:
-  "!nat. nat < length A --> x : free_tv (A!nat) --> x : free_tv A"
+  "\<forall>nat. nat < length A \<longrightarrow> x : free_tv (A!nat) \<longrightarrow> x : free_tv A"
 apply (induct A)
 apply simp
 apply (rule allI)
@@ -336,37 +336,37 @@ text
    occurring in the type structure *}
 
 lemma typ_substitutions_only_on_free_variables: 
-  "(!x:free_tv t. (S x) = (S' x)) \<Longrightarrow> $ S (t::typ) = $ S' t"
+  "(\<forall>x\<in>free_tv t. (S x) = (S' x)) \<Longrightarrow> $ S (t::typ) = $ S' t"
   by (induct t) simp_all
 
-lemma eq_free_eq_subst_te: "(!n. n:(free_tv t) --> S1 n = S2 n) ==> $ S1 (t::typ) = $ S2 t"
+lemma eq_free_eq_subst_te: "(\<forall>n. n\<in>(free_tv t) \<longrightarrow> S1 n = S2 n) \<Longrightarrow> $ S1 (t::typ) = $ S2 t"
 apply (rule typ_substitutions_only_on_free_variables)
 apply simp
 done
 
 lemma scheme_substitutions_only_on_free_variables:
-  "(!x:free_tv sch. (S x) = (S' x)) \<Longrightarrow> $ S (sch::type_scheme) = $ S' sch"
+  "(\<forall>x\<in>free_tv sch. (S x) = (S' x)) \<Longrightarrow> $ S (sch::type_scheme) = $ S' sch"
   by (induct sch) simp_all
 
 lemma eq_free_eq_subst_type_scheme: 
-  "(!n. n:(free_tv sch) --> S1 n = S2 n) ==> $ S1 (sch::type_scheme) = $ S2 sch"
+  "(\<forall>n. n\<in>(free_tv sch) \<longrightarrow> S1 n = S2 n) \<Longrightarrow> $ S1 (sch::type_scheme) = $ S2 sch"
 apply (rule scheme_substitutions_only_on_free_variables)
 apply simp
 done
 
 lemma eq_free_eq_subst_scheme_list:
-  "(!n. n:(free_tv A) --> S1 n = S2 n) \<Longrightarrow> $S1 (A::type_scheme list) = $S2 A"
+  "(\<forall>n. n\<in>(free_tv A) \<longrightarrow> S1 n = S2 n) \<Longrightarrow> $S1 (A::type_scheme list) = $S2 A"
 proof (induct A)
   case Nil then show ?case by fastforce
 next
   case Cons then show ?case by (fastforce intro: eq_free_eq_subst_type_scheme)
 qed
 
-lemma weaken_asm_Un: "((!x:A. (P x)) --> Q) ==> ((!x:A Un B. (P x)) --> Q)"
+lemma weaken_asm_Un: "((\<forall>x\<in>A. (P x)) \<longrightarrow> Q) \<Longrightarrow> ((\<forall>x\<in>A \<union> B. (P x)) \<longrightarrow> Q)"
   by fast
 
 lemma scheme_list_substitutions_only_on_free_variables [rule_format]:
-  "(!x:free_tv A. (S x) = (S' x)) --> $ S (A::type_scheme list) = $ S' A"
+  "(\<forall>x\<in>free_tv A. (S x) = (S' x)) \<longrightarrow> $ S (A::type_scheme list) = $ S' A"
 apply (induct_tac A)
 apply simp
 apply simp
@@ -380,7 +380,7 @@ lemma eq_subst_te_eq_free:
   by (induct t) auto
 
 lemma eq_subst_type_scheme_eq_free [rule_format]: 
-  "$ S1 (sch::type_scheme) = $ S2 sch --> n:(free_tv sch) --> S1 n = S2 n"
+  "$ S1 (sch::type_scheme) = $ S2 sch \<longrightarrow> n:(free_tv sch) \<longrightarrow> S1 n = S2 n"
 apply (induct_tac "sch")
 (* case TVar n *)
 apply simp
@@ -402,17 +402,17 @@ next
   then show ?case by (fastforce intro: eq_subst_type_scheme_eq_free)
 qed
 
-lemma codD: "v : cod S ==> v : free_tv S"
+lemma codD: "v : cod S \<Longrightarrow> v : free_tv S"
   unfolding free_tv_subst by blast
 
-lemma not_free_impl_id: "x ~: free_tv S ==> S x = TVar x"
+lemma not_free_impl_id: "x \<notin> free_tv S \<Longrightarrow> S x = TVar x"
   unfolding free_tv_subst dom_def by blast
 
 lemma free_tv_le_new_tv: "[| new_tv n t; m:free_tv t |] ==> m<n"
   unfolding new_tv_def by blast
 
 lemma cod_app_subst [simp]:
-  "[| v : free_tv(S n); v~=n |] ==> v : cod S"
+  "[| v : free_tv(S n); v\<noteq>n |] ==> v : cod S"
 apply (unfold dom_def cod_def UNION_eq Bex_def)
 apply (simp (no_asm))
 apply (safe intro!: exI)
@@ -420,13 +420,13 @@ prefer 2 apply (assumption)
 apply simp
 done
 
-lemma free_tv_subst_var: "free_tv (S (v::nat)) <= insert v (cod S)"
+lemma free_tv_subst_var: "free_tv (S (v::nat)) \<subseteq> insert v (cod S)"
 apply (cases "v:dom S")
 apply (fastforce simp add: cod_def)
 apply (fastforce simp add: dom_def)
 done
 
-lemma free_tv_app_subst_te: "free_tv ($ S (t::typ)) <= cod S Un free_tv t"
+lemma free_tv_app_subst_te: "free_tv ($ S (t::typ)) \<subseteq> cod S Un free_tv t"
 proof (induct t)
   case (TVar n) then show ?case by (simp add: free_tv_subst_var)
 next
@@ -434,7 +434,7 @@ next
 qed
 
 lemma free_tv_app_subst_type_scheme:
-    "free_tv ($ S (sch::type_scheme)) <= cod S Un free_tv sch"
+    "free_tv ($ S (sch::type_scheme)) \<subseteq> cod S Un free_tv sch"
 proof (induct sch)
   case (FVar n)
   then show ?case by (simp add: free_tv_subst_var)
@@ -446,7 +446,7 @@ next
   then show ?case by fastforce
 qed
 
-lemma free_tv_app_subst_scheme_list: "free_tv ($ S (A::type_scheme list)) <= cod S Un free_tv A"
+lemma free_tv_app_subst_scheme_list: "free_tv ($ S (A::type_scheme list)) \<subseteq> cod S Un free_tv A"
 proof (induct A)
   case Nil then show ?case by simp
 next
@@ -456,26 +456,26 @@ next
 qed
 
 lemma free_tv_comp_subst: 
-  "free_tv (%u::nat. $ s1 (s2 u) :: typ) <=    
+  "free_tv (\<lambda>u::nat. $ s1 (s2 u) :: typ) \<subseteq>    
     free_tv s1 Un free_tv s2"
   unfolding free_tv_subst dom_def
   by (force simp add: cod_def dom_def
     dest!:free_tv_app_subst_te [THEN subsetD])
 
 lemma free_tv_o_subst: 
-    "free_tv ($ S1 o S2) <= free_tv S1 Un free_tv (S2 :: nat => typ)"
+    "free_tv ($ S1 \<circ> S2) \<subseteq> free_tv S1 Un free_tv (S2 :: nat => typ)"
   unfolding o_def by (rule free_tv_comp_subst)
 
 lemma free_tv_of_substitutions_extend_to_types:
-    "n : free_tv t \<Longrightarrow> free_tv (S n) <= free_tv ($ S t::typ)"
+    "n : free_tv t \<Longrightarrow> free_tv (S n) \<subseteq> free_tv ($ S t::typ)"
   by (induct t) auto
 
 lemma free_tv_of_substitutions_extend_to_schemes:
-    "n : free_tv sch \<Longrightarrow> free_tv (S n) <= free_tv ($ S sch::type_scheme)"
+    "n : free_tv sch \<Longrightarrow> free_tv (S n) \<subseteq> free_tv ($ S sch::type_scheme)"
   by (induct sch) auto
 
 lemma free_tv_of_substitutions_extend_to_scheme_lists [simp]:
-    "n : free_tv A \<Longrightarrow> free_tv (S n) <= free_tv ($ S A::type_scheme list)"
+    "n : free_tv A \<Longrightarrow> free_tv (S n) \<subseteq> free_tv ($ S A::type_scheme list)"
   by (induct A) (auto dest: free_tv_of_substitutions_extend_to_schemes)
 
 lemma free_tv_ML_scheme:
@@ -508,8 +508,8 @@ lemma bound_tv_subst_scheme_list [simp]:
 \<comment> \<open>lemmata for @{text new_tv}\<close>
 
 lemma new_tv_subst: 
-  "new_tv n S = ((!m. n <= m --> (S m = TVar m)) &  
-                 (! l. l < n --> new_tv n (S l) ))"
+  "new_tv n S = ((\<forall>m. n \<le> m \<longrightarrow> (S m = TVar m)) \<and>  
+                 (\<forall>l. l < n \<longrightarrow> new_tv n (S l) ))"
 
 apply (unfold new_tv_def)
 apply (safe)
@@ -518,7 +518,7 @@ apply (safe)
  apply (subgoal_tac "m:cod S | S l = TVar l")
   apply safe
    apply (fastforce dest: UnI2 simp add: free_tv_subst)
-  apply (drule_tac P = "%x. m:free_tv x" in subst , assumption)
+  apply (drule_tac P = "\<lambda>x. m:free_tv x" in subst , assumption)
   apply simp
  apply (fastforce simp add: free_tv_subst cod_def dom_def)
 (* <== *)
@@ -527,26 +527,26 @@ apply safe
 apply (metis not_le_imp_less)+
 done
 
-lemma new_tv_list: "new_tv n x = (!y:set x. new_tv n y)"
+lemma new_tv_list: "new_tv n x = (\<forall>y\<in>set x. new_tv n y)"
   by (induct x) simp_all
 
 \<comment> \<open>substitution affects only variables occurring freely\<close>
 lemma subst_te_new_tv [simp]:
-    "new_tv n (t::typ) --> $(%x. if x=n then t' else S x) t = $S t"
+    "new_tv n (t::typ) \<longrightarrow> $(\<lambda>x. if x=n then t' else S x) t = $S t"
   by (induct t) simp_all
 
 lemma subst_te_new_type_scheme [simp]:
-    "new_tv n (sch::type_scheme) \<Longrightarrow> $(%x. if x=n then sch' else S x) sch = $S sch"
+    "new_tv n (sch::type_scheme) \<Longrightarrow> $(\<lambda>x. if x=n then sch' else S x) sch = $S sch"
   by (induct sch) simp_all
 
 lemma subst_tel_new_scheme_list [simp]:
-    "new_tv n (A::type_scheme list) \<Longrightarrow> $(%x. if x=n then t else S x) A = $S A"
+    "new_tv n (A::type_scheme list) \<Longrightarrow> $(\<lambda>x. if x=n then t else S x) A = $S A"
   by (induct A) simp_all
 
 
 \<comment> \<open>all greater variables are also new\<close>
 lemma new_tv_le: 
-  "n<=m ==> new_tv n t ==> new_tv m t"
+  "n\<le>m \<Longrightarrow> new_tv n t \<Longrightarrow> new_tv m t"
 apply (unfold new_tv_def)
 apply safe
 apply (drule spec)
@@ -557,13 +557,13 @@ done
 lemma [simp]: "new_tv n t \<Longrightarrow> new_tv (Suc n) t"
   by (rule lessI [THEN less_imp_le [THEN new_tv_le]])
 
-lemma new_tv_typ_le: "n<=m ==> new_tv n (t::typ) ==> new_tv m t"
+lemma new_tv_typ_le: "n\<le>m \<Longrightarrow> new_tv n (t::typ) \<Longrightarrow> new_tv m t"
   by (simp add: new_tv_le)
 
-lemma new_scheme_list_le: "n<=m ==> new_tv n (A::type_scheme list) ==> new_tv m A"
+lemma new_scheme_list_le: "n\<le>m \<Longrightarrow> new_tv n (A::type_scheme list) \<Longrightarrow> new_tv m A"
   by (simp add: new_tv_le)
 
-lemma new_tv_subst_le: "n<=m ==> new_tv n (S::subst) ==> new_tv m S"
+lemma new_tv_subst_le: "n\<le>m \<Longrightarrow> new_tv n (S::subst) \<Longrightarrow> new_tv m S"
   by (simp add: new_tv_le)
 
 \<comment> \<open>@{text new_tv} property remains if a substitution is applied\<close>
@@ -576,7 +576,7 @@ lemma new_tv_subst_te [simp]:
   by (induct t) (auto simp add: new_tv_subst)
 
 lemma new_tv_subst_type_scheme [rule_format, simp]: 
-  "new_tv n S --> new_tv n (sch::type_scheme) --> new_tv n ($ S sch)"
+  "new_tv n S \<longrightarrow> new_tv n (sch::type_scheme) \<longrightarrow> new_tv n ($ S sch)"
 apply (induct sch)
 apply (simp_all)
 apply (unfold new_tv_def)
@@ -593,7 +593,7 @@ lemma new_tv_subst_scheme_list [simp]:
     "new_tv n S \<Longrightarrow> new_tv n (A::type_scheme list) \<Longrightarrow> new_tv n ($ S A)"
   by (induct A) auto
 
-lemma new_tv_Suc_list: "new_tv n A --> new_tv (Suc n) ((TVar n)#A)"
+lemma new_tv_Suc_list: "new_tv n A \<longrightarrow> new_tv (Suc n) ((TVar n)#A)"
   by (simp add: new_tv_list)
 
 lemma new_tv_only_depends_on_free_tv_type_scheme:
@@ -607,7 +607,7 @@ lemma new_tv_only_depends_on_free_tv_scheme_list:
   unfolding new_tv_def by simp
 
 lemma new_tv_nth_nat_A [rule_format]: 
-  "!nat. nat < length A --> new_tv n A --> (new_tv n (A!nat))"
+  "\<forall>nat. nat < length A \<longrightarrow> new_tv n A \<longrightarrow> (new_tv n (A!nat))"
 apply (unfold new_tv_def)
 apply (induct A)
 apply simp
@@ -621,19 +621,19 @@ done
 
 \<comment> \<open>composition of substitutions preserves @{text new_tv} proposition\<close>
 lemma new_tv_subst_comp_1 [simp]: 
-  "[| new_tv n (S::subst); new_tv n R |] ==> new_tv n (($ R) o S)"
+  "[| new_tv n (S::subst); new_tv n R |] ==> new_tv n (($ R) \<circ> S)"
   by (simp add: new_tv_subst)
 
 lemma new_tv_subst_comp_2 [simp]:
-  "[| new_tv n (S::subst); new_tv n R |] ==> new_tv n (%v.$ R (S v))"
+  "[| new_tv n (S::subst); new_tv n R |] ==> new_tv n (\<lambda>v.$ R (S v))"
   by (simp add: new_tv_subst)
 
 \<comment> \<open>new type variables do not occur freely in a type structure\<close>
 lemma new_tv_not_free_tv [simp]:
-    "new_tv n A ==> n~:(free_tv A)"
+    "new_tv n A \<Longrightarrow> n\<notin>(free_tv A)"
   by (auto simp add: new_tv_def)
 
-lemma fresh_variable_types [simp]: "!!t::typ. ? n. (new_tv n t)"
+lemma fresh_variable_types [simp]: "\<And>t::typ. \<exists>n. (new_tv n t)"
 apply (unfold new_tv_def)
 apply (induct_tac t)
 apply (rename_tac nat)
@@ -646,7 +646,7 @@ apply (simp add: less_max_iff_disj)
 done
 
 lemma fresh_variable_type_schemes [simp]:
-  "!!sch::type_scheme. ? n. (new_tv n sch)"
+  "\<And>sch::type_scheme. \<exists>n. (new_tv n sch)"
 apply (unfold new_tv_def)
 apply (induct_tac sch)
 apply (rename_tac nat)
@@ -662,7 +662,7 @@ apply (simp add: less_max_iff_disj)
 done
 
 lemma fresh_variable_type_scheme_lists [simp]: 
-  "!!A::type_scheme list. ? n. (new_tv n A)"
+  "\<And>A::type_scheme list. \<exists>n. (new_tv n A)"
 apply (induct_tac A)
 apply (simp (no_asm))
 apply (simp (no_asm))
@@ -671,37 +671,37 @@ apply (cut_tac sch = "a" in fresh_variable_type_schemes)
 apply (erule exE)
 apply (rename_tac "n'")
 apply (rule_tac x = " (max n n') " in exI)
-apply (subgoal_tac "n <= (max n n') ")
-apply (subgoal_tac "n' <= (max n n') ")
+apply (subgoal_tac "n \<le> (max n n') ")
+apply (subgoal_tac "n' \<le> (max n n') ")
 apply (fast dest: new_tv_le)
 apply (simp_all add: le_max_iff_disj)
 done
 
 lemma make_one_new_out_of_two: 
-  "[| ? n1. (new_tv n1 x); ? n2. (new_tv n2 y)|] ==> ? n. (new_tv n x) & (new_tv n y)"
+  "[| \<exists>n1. (new_tv n1 x); \<exists>n2. (new_tv n2 y)|] ==> \<exists>n. (new_tv n x) \<and> (new_tv n y)"
 apply (erule exE)+
 apply (rename_tac "n1" "n2")
 apply (rule_tac x = " (max n1 n2) " in exI)
-apply (subgoal_tac "n1 <= max n1 n2")
-apply (subgoal_tac "n2 <= max n1 n2")
+apply (subgoal_tac "n1 \<le> max n1 n2")
+apply (subgoal_tac "n2 \<le> max n1 n2")
 apply (fast dest: new_tv_le)
 apply (simp_all (no_asm) add: le_max_iff_disj)
 done
 
 lemma ex_fresh_variable: 
-  "!!(A::type_scheme list) (A'::type_scheme list) (t::typ) (t'::typ).  
-          ? n. (new_tv n A) & (new_tv n A') & (new_tv n t) & (new_tv n t')"
+  "\<And>(A::type_scheme list) (A'::type_scheme list) (t::typ) (t'::typ).  
+          \<exists>n. (new_tv n A) \<and> (new_tv n A') \<and> (new_tv n t) \<and> (new_tv n t')"
 apply (cut_tac t = "t" in fresh_variable_types)
 apply (cut_tac t = "t'" in fresh_variable_types)
 apply (drule make_one_new_out_of_two)
 apply assumption
-apply (erule_tac V = "? n. new_tv n t'" in thin_rl)
+apply (erule_tac V = "\<exists>n. new_tv n t'" in thin_rl)
 apply (cut_tac A = "A" in fresh_variable_type_scheme_lists)
 apply (cut_tac A = "A'" in fresh_variable_type_scheme_lists)
 apply (rotate_tac 1)
 apply (drule make_one_new_out_of_two)
 apply assumption
-apply (erule_tac V = "? n. new_tv n A'" in thin_rl)
+apply (erule_tac V = "\<exists>n. new_tv n A'" in thin_rl)
 apply (erule exE)+
 apply (rename_tac n2 n1)
 apply (rule_tac x = " (max n1 n2) " in exI)
@@ -721,7 +721,7 @@ done
 (* lemmata for substitutions *)
 
 lemma length_app_subst_list [simp]:
-   "!!A:: ('a::type_struct) list. length ($ S A) = length A"
+   "\<And>A:: ('a::type_struct) list. length ($ S A) = length A"
   unfolding app_subst_list by simp
 
 lemma subst_TVar_scheme [simp]:
@@ -735,7 +735,7 @@ lemma subst_TVar_scheme_list [simp]:
   by (induct A) (simp_all add: app_subst_list)
 
 \<comment> \<open>application of @{text id_subst} does not change type expression\<close>
-lemma app_subst_id_te [simp]: "$ id_subst = (%t::typ. t)"
+lemma app_subst_id_te [simp]: "$ id_subst = (\<lambda>t::typ. t)"
 apply (unfold id_subst_def)
 apply (rule ext)
 apply (induct_tac "t")
@@ -743,7 +743,7 @@ apply simp_all
 done
 
 lemma app_subst_id_type_scheme [simp]:
-  "$ id_subst = (%sch::type_scheme. sch)"
+  "$ id_subst = (\<lambda>sch::type_scheme. sch)"
 apply (unfold id_subst_def)
 apply (rule ext)
 apply (induct_tac "sch")
@@ -752,7 +752,7 @@ done
 
 \<comment> \<open>application of @{text id_subst} does not change list of type expressions\<close>
 lemma app_subst_id_tel [simp]: 
-  "$ id_subst = (%A::type_scheme list. A)"
+  "$ id_subst = (\<lambda>A::type_scheme list. A)"
 apply (unfold app_subst_list)
 apply (rule ext)
 apply (induct_tac "A")
@@ -770,18 +770,18 @@ lemma id_subst_A [simp]:
   by (induct A) simp_all
 
 \<comment> \<open>composition of substitutions\<close>
-lemma o_id_subst [simp]: "$S o id_subst = S"
+lemma o_id_subst [simp]: "$S \<circ> id_subst = S"
   unfolding id_subst_def o_def by simp
 
-lemma subst_comp_te: "$ R ($ S t::typ) = $ (%x. $ R (S x) ) t"
+lemma subst_comp_te: "$ R ($ S t::typ) = $ (\<lambda>x. $ R (S x) ) t"
   by (induct t) simp_all
 
 lemma subst_comp_type_scheme: 
-  "$ R ($ S sch::type_scheme) = $ (%x. $ R (S x) ) sch"
+  "$ R ($ S sch::type_scheme) = $ (\<lambda>x. $ R (S x) ) sch"
   by (induct sch) simp_all
 
 lemma subst_comp_scheme_list: 
-  "$ R ($ S A::type_scheme list) = $ (%x. $ R (S x)) A"
+  "$ R ($ S A::type_scheme list) = $ (\<lambda>x. $ R (S x)) A"
 unfolding app_subst_list
 proof (induct A)
   case Nil then show ?case by simp
@@ -792,21 +792,21 @@ qed
 
 lemma subst_id_on_type_scheme_list': 
   fixes A :: "type_scheme list"
-  shows "!x : free_tv A. S x = (TVar x) ==> $ S A = $ id_subst A"
+  shows "\<forall>x \<in> free_tv A. S x = (TVar x) \<Longrightarrow> $ S A = $ id_subst A"
 apply (rule scheme_list_substitutions_only_on_free_variables)
 apply (simp add: id_subst_def)
 done
 
 lemma subst_id_on_type_scheme_list: 
   fixes A :: "type_scheme list"
-  shows "!x : free_tv A. S x = (TVar x) ==> $ S A = A"
+  shows "\<forall>x \<in> free_tv A. S x = (TVar x) \<Longrightarrow> $ S A = A"
 apply (subst subst_id_on_type_scheme_list')
 apply assumption
 apply simp
 done
 
 lemma nth_subst [rule_format]: 
-  "!n. n < length A --> ($ S A)!n = $S (A!n)"
+  "\<forall>n. n < length A \<longrightarrow> ($ S A)!n = $S (A!n)"
 apply (induct A)
 apply simp
 apply (rule allI)
